nondeterministic_dataflow/Eval.thy
@@ -3,6 +3,15 @@ imports BNA_Operators
   CSet_LList_Impl
 begin
 
+fun show_IO where
+  "show_IO showI showO show (Out p x) = STR ''Out '' + showO p + STR '' '' + show x"
+| "show_IO showI showO show (Inp p x) = STR ''Inp '' + showI p + STR '' '' + show x"
+| "show_IO showI showO show Tau = STR ''Tau''"
+
+definition show_1 where "show_1 (x :: 1) = STR ''1''"
+definition show_11 where "show_11 = show_sum show_1 show_1"
+definition show_2 where "show_2 (x :: 2) = (if x = 1 then STR ''1'' else STR ''2'')"
+
 fun eval :: "nat \<Rightarrow> ('i, 'o, 'd :: countable) op \<Rightarrow> (('i, 'o, 'd) IO list \<times> ('i, 'o, 'd) op) cset"  where
   "eval 0 op = {|([], op)|}"
 | "eval (Suc n) (Read p f) = cUnion (cimage (\<lambda>x. cimage (\<lambda>(t, op). (Inp p x # t, op)) (eval n (f x))) (cUNIV :: 'd cset))"
@@ -14,11 +23,13 @@ definition W42 :: "(2,1,nat) op" where "W42 = Write end_op 1 42"
 definition CP :: "(1,1,bool) op" where "CP = Read 1 (\<lambda>x. Write end_op 1 x)"
 corec cp_op :: "(1,1,bool) op" where "cp_op = Read 1 (\<lambda>x. Write cp_op 1 x)"
 
-value [GHC] "force_cset undefined 10 (cimage fst (eval 10 W42))"
-value [GHC] "force_cset undefined 10 (cimage fst (eval 10 CP))"
-value [GHC] "force_cset undefined 100 (cimage fst (eval 10 cp_op))"
-value [GHC] "force_cset undefined 100 (cimage fst (eval 1000 (CP \<bullet> CP)))"
-value [GHC] "force_cset undefined 100 (cimage fst (eval 10 (cp_op \<bullet> cp_op)))"
-value [GHC] "force_cset undefined 100 (cimage fst (eval 10 (cp_op \<parallel> cp_op)))"
+value [GHC] "force_cset (show_list (show_IO show_2 show_1 show_nat)) 10 (cimage fst (eval 10 W42))"
+value [GHC] "force_cset (show_list (show_IO show_1 show_1 show_bool)) 10 (cimage fst (eval 10 CP))"
+value [GHC] "force_cset (show_list (show_IO show_1 show_1 show_bool)) 100 (cimage fst (eval 10 cp_op))"
+value [GHC] "force_cset (show_list (show_IO show_1 show_1 show_bool)) 100 (cimage fst (eval 1000 (CP \<bullet> CP)))"
+value [GHC] "force_cset (show_list (show_IO show_1 show_1 show_bool)) 100 (cimage fst (eval 10 (cp_op \<bullet> cp_op)))"
+value [GHC] "force_cset (show_list (show_IO show_11 show_11 show_bool)) 100 (cimage fst (eval 10 (cp_op \<parallel> cp_op)))"
+definition bar where "bar = cis_empty (force_cset (show_list (show_IO show_1 show_1 show_bool)) 200 (cimage fst (eval 200 (cp_op \<bullet> cp_op))))"
+export_code bar in Haskell module_name Bar
 
 end
